Letâ€™s see the algebraic proof of the notion that selecting $p$ -many elements out of a set of $n$ is the same as omitting n-p many elements.

For starters, recall the combination formula:

$$
C ( n , p ) = { \frac { n ! } { ( n - p ) ! p ! } }
$$

If we plug in $n - p$ for $p ,$ we get the following:

$$
\frac { n ! } { - p ) ) ! ( n - p ) ! } = \frac { n ! } { ( n - n + p ) ) ! ( n - p ) ! } = \frac { n ! } { p ! ( n - p ) ! } =
$$

Therefore, we can conclude that $\pmb { C } ( \pmb { n } , \pmb { p } ) = \pmb { C } ( \pmb { n } , \pmb { n } - \pmb { p } )$ .